\documentclass{article}
\usepackage[utf8]{inputenc}
\usepackage[top=1cm,bottom=1cm,left=1cm,right=1cm]{geometry}
\usepackage{amsmath}
\usepackage{physics}

\renewcommand{\phi}{\varphi}

\pagenumbering{gobble}

\begin{document}

\begin{align*}
  % Cartesian coordinates
  x_i &= \sum_{k=1}^i l_k \sin(\phi_k) \\
  y_i &= - \sum_{k=1}^i l_k \cos(\phi_k) \\
  \dot x_i &= \sum_{k=1}^i l_k \cos(\phi_k) \dot\phi_k \\
  \dot y_i &= \sum_{k=1}^i l_k \sin(\phi_k) \dot\phi_k \\
\end{align*}
\begin{align*}
  % Energies
  U &= \sum_{i=1}^n m_i g y_i \\
  T &= \sum_{i=1}^n \frac{m_i}{2} \pqty{\dot x_i^2 + \dot y_i^2} \\
\end{align*}
\begin{align*}
  % Lagrangian
  L &= T - U \\
    &= \sum_{i=1}^n \frac{m_i}{2} \pqty{\dot x_i^2 + \dot y_i^2} - \sum_{i=1}^n m_i g y_i \\
    &= \sum_{i=1}^n m_i \pqty{\frac{1}{2} \pqty{\dot x_i^2 + \dot y_i^2} - g y_i} \\
    &= \sum_{i=1}^n m_i \pqty{\frac{1}{2} \pqty{{\pqty{\sum_{k=1}^i l_k \cos(\phi_k) \dot\phi_k}}^2 + {\pqty{\sum_{k=1}^i l_k \sin(\phi_k) \dot\phi_k}}^2} + g \sum_{k=1}^i l_k \cos(\phi_k)} \\
\end{align*}
\begin{align*}
  % Lagrangian derivatives
  \pdv{L}{\phi_j} &= \sum_{i=1}^n m_i \pqty{-l_j \sin(\phi_j) \dot\phi_j \sum_{k=1}^i l_k \cos(\phi_k) \dot\phi_k + l_j \cos(\phi_j) \dot\phi_j \sum_{k=1}^i l_k \sin(\phi_k) \dot\phi_k - g \sum_{k=1}^i l_k \sin(\phi_k)} \\
                  &= \sum_{i=1}^n m_i \sum_{k=1}^i l_k \pqty{-l_j \sin(\phi_j) \dot\phi_j \cos(\phi_k) \dot\phi_k + l_j \cos(\phi_j) \dot\phi_j \sin(\phi_k) \dot\phi_k - g \sin(\phi_k)} \\
                  &= \sum_{i=1}^n m_i \sum_{k=1}^i l_k \pqty{l_j \sin(\phi_k - \phi_j) \dot\phi_j \dot\phi_k - g \sin(\phi_k)} \\
  \pdv{L}{\dot\phi_j} &= \sum_{i=1}^n m_i \pqty{l_j \cos(\phi_j) \sum_{k=1}^i l_k \cos(\phi_k) \dot\phi_k + l_j \sin(\phi_j) \sum_{k=1}^i l_k \sin(\phi_k) \dot\phi_k} \\
                      &= \sum_{i=1}^n m_i l_j \sum_{k=1}^i \pqty{l_k \cos(\phi_j) \cos(\phi_k) \dot\phi_k + l_k \sin(\phi_j) l_k \sin(\phi_k) \dot\phi_k} \\
                      &= \sum_{i=1}^n m_i l_j \sum_{k=1}^i l_k \cos(\phi_k - \phi_j) \dot\phi_k \\
  \dv{t} \pdv{L}{\dot\phi_j} &= \sum_{i=1}^n m_i l_j \sum_{k=1}^i l_k \pqty{\cos(\phi_k - \phi_j) \ddot\phi_k - \sin(\phi_k - \phi_j)(\dot\phi_k - \dot\phi_j)\dot\phi_k} \\
                             &= \sum_{i=j}^n m_i l_j^2 \ddot\phi_j + \sum_{i=1}^n m_i l_j \sum_{\substack{k=1\\k \neq j}}^i l_k \pqty{\cos(\phi_k - \phi_j) \ddot\phi_k - \sin(\phi_k - \phi_j)(\dot\phi_k - \dot\phi_j)\dot\phi_k} \\
\end{align*}
\begin{align*}
  % Lagrangian equation
  \sum_{i=j}^n m_i l_j^2 \ddot\phi_j &+ \sum_{i=1}^n m_i l_j \sum_{\substack{k=1\\k \neq j}}^i l_k \pqty{\cos(\phi_k - \phi_j) \ddot\phi_k - \sin(\phi_k - \phi_j)(\dot\phi_k - \dot\phi_j)\dot\phi_k} = \sum_{i=1}^n m_i \sum_{k=1}^i l_k \pqty{l_j \sin(\phi_k - \phi_j) \dot\phi_j \dot\phi_k - g \sin(\phi_k)} \\
  \sum_{i=j}^n m_i l_j^2 \ddot\phi_j &= \sum_{i=1}^n m_i \sum_{k=1}^i l_k \pqty{l_j \sin(\phi_k - \phi_j) \dot\phi_j \dot\phi_k - g \sin(\phi_k)} - \sum_{i=1}^n m_i l_j \sum_{\substack{k=1\\k \neq j}}^i l_k \pqty{\cos(\phi_k - \phi_j) \ddot\phi_k - \sin(\phi_k - \phi_j)(\dot\phi_k - \dot\phi_j)\dot\phi_k} \\
  \sum_{i=j}^n m_i l_j^2 \ddot\phi_j &= \sum_{i=1}^n m_i \sum_{\substack{k=1\\k \neq j}}^i l_k \pqty{l_j \pqty{\sin(\phi_k - \phi_j) \dot\phi_j \dot\phi_k - \cos(\phi_k - \phi_j) \ddot\phi_k + \sin(\phi_k - \phi_j)(\dot\phi_k - \dot\phi_j)\dot\phi_k} - g \sin(\phi_k)} - \sum_{i=j}^n m_i l_j g \sin(\phi_k) \\
  \sum_{i=j}^n m_i l_j^2 \ddot\phi_j &= \sum_{i=1}^n m_i \sum_{\substack{k=1\\k \neq j}}^i l_k \pqty{l_j \pqty{\sin(\phi_k - \phi_j) \dot\phi_j^2 - \cos(\phi_k - \phi_j) \ddot\phi_k} - g \sin(\phi_k)} - \sum_{i=j}^n m_i l_j g \sin(\phi_k) \\
  \ddot\phi_j &= \frac{\sum_{i=1}^n m_i \sum_{\substack{k=1\\k \neq j}}^i l_k \pqty{l_j \pqty{\sin(\phi_k - \phi_j) \dot\phi_j^2 - \cos(\phi_k - \phi_j) \ddot\phi_k} - g \sin(\phi_k)} - \sum_{i=j}^n m_i l_j g \sin(\phi_k)}{\sum_{i=j}^n m_i l_j^2} \\
\end{align*}

\end{document}
